Gossip/Error/Examples.lean
@@ -1,0 +1,91 @@
+import Gossip.Error.Decide
+import Gossip.Error.SemProp
+
+open Error Form Call Role
+
+example :
+  let S : @Dist 3 := fun _ => true
+  let σ : @OSequence 3 := ⟨[], by simp⟩
+  S⌈σ⌉ ⊧ .Top := by
+    -- decide -- mmwah?!
+    sorry
+
+#eval
+  let S : @Dist 3 := fun _ => true
+  let σ : @OSequence 3 := ⟨[ ⌜ 0 1^1 ⌝ ], by simp [maxOne]⟩
+  S⌈σ⌉ ⊧ (⟨1,true⟩ @ 0)
+
+def goalForm (a b : @Agent n) : @Form n :=
+      (¬'(b @ a)) ⋀ (K a (b @ b))
+
+def validAt {n : Nat} (k : Nat) (φ : @Form n) : Prop :=
+  ∀ S, ∀ σ : { σ : @OSequence n // σ.length = k } , S⌈σ.1⌉ ⊧ φ
+
+instance instDecValidAt : Decidable (@validAt n k φ) := by
+  unfold validAt
+  refine Decidable.forall_of_list_mem Dist.all_spec (fun S => ?_)
+  refine Decidable.forall_of_list_mem OSequence.fixLen_all_spec (fun σ => ?_)
+  exact instDecEval
+
+-- #eval (@Call.all 3).length
+-- #eval (3 * 3) + (3* 3 * 3) + (3* 3 * 3)
+
+-- #eval
+--   (@OSequence.fixLen_all 3 1).length
+
+-- #eval
+--   @validAt 3 2 (¬' goalForm 0 1)
+
+/-! ## Examples -/
+
+/-- Initial distribution with all values set to true. -/
+def ini (n : Nat) : @Dist n := fun _ => true
+
+#eval
+  let a : @Agent 2 := 0
+  let b : @Agent 2 := 1
+  eval (ini 2) ⟨[ ⌜a b⌝ ], by simp [maxOne]⟩ $
+      (    b @ a)  -- a believes b
+    ⋀ (¬'(‾b @ a)) -- (and does not believe not-b)
+    ⋀ (   b @ b)   -- correctly,
+    ⋀ (¬'(Kv a b)) -- but a does not *know* the value of b.
+
+-- FIXME: make it easier to define a state / give a sequence without writing `simp [maxOne]`.
+
+/-- Correct belief need not imply knowledge: given `ini 2`, after an initial call
+`ab` agent `a` correclty believes `b`, but a does not know the secret of `b`, because `a`
+also considers it possible that the call was `a b^b` instead. -/
+lemma example_correct_belief_does_not_imply_knowledege (a b : Agent) (h : a ≠ b) :
+    eval (ini 2) ⟨[ ⌜a b⌝ ], by simp [maxOne]⟩ $
+      (    b @ a)  -- a believes b
+    ⋀ (¬'(‾b @ a)) -- (and does not believe not-b)
+    ⋀ (   b @ b)   -- correctly,
+    ⋀ (¬'(Kv a b)) -- but a does not *know* the value of b.
+    := by
+  unfold ini
+  unfold eval
+  constructor
+  · simp [eval, resultSet, contribSet]
+    constructor
+    · use ini 2
+      unfold ini
+      simp only [and_true]
+      use ⟨[], maxOne_nil⟩
+      simp
+    · refine ⟨_, _, ⟨ ⟨ ?_, equiv_refl⟩ , ?_ ⟩  ⟩ <;> simp
+      use ⌜a b⌝
+      simp [contribSet, maxOne]
+  · unfold eval
+    constructor
+    · simp [eval, resultSet, contribSet]
+    · simp_all [eval]
+      use (ini 2).switch b
+      simp only [Dist.switch, ini, Bool.not_true, Bool.if_true_right, Bool.or_false, ↓reduceIte,
+        true_and]
+      constructor
+      · use ⟨[⌜a b^b⌝], by simp [maxOne]⟩
+        simp_all [equiv, roleOfIn, contribSet, invert, Call.pair]
+      · use ini 2
+        simp only [ini, and_true]
+        use ⟨[⌜a b⌝], by simp [maxOne]⟩
+        simp_all [equiv, roleOfIn, contribSet, Call.pair, ini]
